verified/lowstar_to_cstar_proof.lean
@@ -44,27 +44,27 @@ inductive back_stmt : ∀ {X : Type u},
   back_stmt names
     ((stmt.decl b e) :: ss)
     (exp.let_in τ le1 le)
-| let_newbuf : ∀ X (names : X → ident) x b n ss e le1 τ le,
-  back_exp names e le1 →
+| let_newbuf : ∀ X (names : X → ident) b ss e x n le1 τ le,
   x = binder.name b →
-  back_stmt (names_cons x names) ss le →
+  back_exp names e le1 →
   transl_typ τ = binder.typ b → -- ehh
+  back_stmt (names_cons x names) ss le →
   back_stmt names
     ((stmt.decl_buf b n) :: (stmt.write_buf (exp.var x) n e) :: ss)
     (exp.let_newbuf n le1 τ le)
-| let_app : ∀ X (names : X → ident) b x τ fn e ss le1 le,
-  back_exp names e le1 →
+| let_app : ∀ X (names : X → ident) b e ss x τ fn le1 le,
   x = binder.name b →
   transl_typ τ = binder.typ b → -- ehh
+  back_exp names e le1 →
   back_stmt (names_cons x names) ss le →
   back_stmt names
     ((stmt.call b fn e) :: ss)
     (exp.let_app τ fn le1 le)
 | let_readbuf : ∀ X (names : X → ident) b x τ e1 e2 ss le1 le2 le,
-  back_exp names e1 le1 →
-  back_exp names e2 le2 →
   x = binder.name b →
   transl_typ τ = binder.typ b → -- ehh
+  back_exp names e1 le1 →
+  back_exp names e2 le2 →
   back_stmt (names_cons x names) ss le →
   back_stmt names
     ((stmt.read b (exp.ptr_add e1 e2)) :: ss)
@@ -77,26 +77,24 @@ inductive back_stmt : ∀ {X : Type u},
   back_stmt names
     ((stmt.write (exp.ptr_add e1 e2) e3) :: ss)
     (exp.writebuf le1 le2 le3 le)
-| withframe : ∀ X (names : X → ident) ss1 ss le1 le,
+| withframe : ∀ X (names : X → ident) ss1 le1,
   back_stmt names ss1 le1 →
-  back_stmt names ss le →
   back_stmt names
-    ((stmt.block ss1) :: ss)
-    (exp.ignore (exp.withframe le1) le)
+    [stmt.block ss1]
+    (exp.withframe le1) -- ?
 | ignore : ∀ X (names : X → ident) e1 ss le1 le,
   back_exp names e1 le1 →
   back_stmt names ss le →
   back_stmt names
     ((stmt.ignore e1) :: ss)
     (exp.ignore le1 le)
-| if_then_else : ∀ X (names : X → ident) e ss1 ss2 ss3 le le1 le2 le3,
+| if_then_else : ∀ X (names : X → ident) e ss1 ss2 le le1 le2,
   back_exp names e le →
   back_stmt names ss1 le1 →
   back_stmt names ss2 le2 →
-  back_stmt names ss3 le3 →
   back_stmt names
-    ((stmt.if_then_else e ss1 ss2) :: ss3)
-    (exp.ignore (exp.if_then_else le le1 le2) le3)
+    [stmt.if_then_else e ss1 ss2]
+    (exp.if_then_else le le1 le2) -- ?
 | exp : ∀ X (names : X → ident) e le,
   back_exp names e le →
   back_stmt names [stmt.return e] le
@@ -467,6 +465,14 @@ do
     (do apply ``(names_cons_injective), try assumption) <|> -- XX
     assumption <|>
     skip
+  | `(fresh_in _ _) :=
+    (do apply ``(fresh_ident_fresh), try assumption) <|>
+    assumption <|>
+    skip
+  | `(names_in _ _) :=
+    (do apply ``(names_in_cons), exact ``(0:nat), assumption) <|>
+    assumption <|>
+    skip
   | `(_ = _) :=
     assumption <|>
     (do symmetry, assumption) <|>
@@ -517,29 +523,39 @@ end
 
 lemma back_transl_stmt_eq {X : Type u}:
   ∀ (e e' : exp X) seen seen' names ss,
+  names_in names seen →
   function.injective names →
   transl_to_stmt seen names e = some (seen', ss) →
   back_stmt names ss e' →
   e = e'
 :=
 begin
-  intros e, induction e; intros e' seen seen' names ss Hinj HT HB;
+  intros e, induction e; intros e' seen seen' names ss Hseen Hinj HT HB;
   simp [transl_to_stmt] at HT;
   try { opt_inv HT with _ H1, cases HB, /- with .. FIXME -/
     rw (back_transl_exp_eq _ _ _ _ Hinj H1), assumption
   },
-  case exp.if_then_else Y e1 e2 e3 {
+  case exp.if_then_else Y e1 e2 e3 ih_1 ih_2 ih_3 e {
     opt_inv HT with ss1 seen1 H1' H1, simp [transl_to_stmt] at H1',
     opt_inv H1' with ss2 seen2 H2' H2, simp [transl_to_stmt] at H2', opt_inv H2',
-    -- cases HB,
-    /- cases HB -/ /- FIXME -/ admit
+    cases HB, case back_stmt.if_then_else e1' e2' e3' He1' He2' He3' {
+      rw (ih_1 e1'); ok, rw (ih_2 e2'); ok, rw (ih_3 e3'),
+      show transl_to_stmt _ _ _ = _, { assumption },
+      show back_stmt _ _ _, { assumption },
+      show names_in _ _, {
+        intro,
+        apply (transl_to_stmt_seen_incl _ _ _ _ _ H1),
+        apply Hseen
+      },
+      assumption
+    }
   },
   case exp.let_in Y τ e1 e2 {
     opt_inv HT with ss1 seen1 H1' H1, simp [transl_to_stmt] at H1', opt_inv H1',
     cases HB, case back_stmt.let_in τ' e1' e2' {
       -- dsimp at *, -- FIXME: do not unfold injective
       rw (ih_1 e1'); ok; try { assumption },
-      rw (ih_2 e2'); ok; [skip, admit],
+      rw (ih_2 e2'); ok; ok, -- FIXME spurious "ident" goal after "apply names_in_cons"
       rw (@transl_typ_injective τ τ'); ok
     }
   },
@@ -554,7 +570,7 @@ begin
     opt_inv HT with ss1 seen1 H1' H1, simp [transl_to_stmt] at H1', opt_inv H1',
     cases HB, case back_stmt.let_app x τ' e1' e2' {
       rw (ih_1 e1'); ok; try { assumption },
-      rw (ih_2 e2'); ok; [skip, admit],
+      rw (ih_2 e2'); ok; ok,
       rw (@transl_typ_injective τ τ'); ok
     }
   },
@@ -562,7 +578,7 @@ begin
     opt_inv HT with ss1 seen1 H1' H1, simp [transl_to_stmt] at H1', opt_inv H1',
     cases HB, case back_stmt.let_newbuf e1' τ' e2' {
       rw (ih_1 e1'); ok; try { assumption },
-      rw (ih_2 e2'); ok; [skip, admit],
+      rw (ih_2 e2'); ok; ok,
       rw (@transl_typ_injective τ τ'); ok
     }
   },
@@ -571,7 +587,7 @@ begin
     cases HB, case back_stmt.let_readbuf x τ' e1' e2' e3' {
       rw (ih_1 e1'); ok; try { assumption },
       rw (ih_2 e2'); ok; try { assumption },
-      rw (ih_3 e3'); ok; [skip, admit],
+      rw (ih_3 e3'); ok; ok,
       rw (@transl_typ_injective τ τ'); ok
     }
   },
@@ -586,12 +602,14 @@ begin
   },
   case exp.withframe Y e {
     opt_inv HT with ss1 seen1 H1' H1, simp [transl_to_stmt] at H1', opt_inv H1',
-    /- cases HB -/ admit
+    cases HB, rw (ih_1 _); ok
   },
   case exp.pop Y e { injection HT }
 end
 
 lemma init : ∀ X seen seen' seen'' (names : X → ident) p lp le ss V,
+  names_in names seen →
+  function.injective names →
   transl_program seen lp = some (seen', p) →
   transl_to_stmt seen' names le = some (seen'', ss) →
   rel p lp names ([], close_vars names V le) ([], V, ss) :=
@@ -599,6 +617,8 @@ begin
   intros X,
   assert Hsteps :
     ∀ le seen seen' (names : X → ident) p lp V ss ss' le',
+    names_in names seen →
+    function.injective names →
     transl_to_stmt seen names le = some (seen', ss) →
     eval_head_exp p V ss ss' →
     back_stmt names ss' le' →
@@ -606,25 +626,24 @@ begin
       ([], close_vars names V le)
       ([], close_vars names V le')
       [],
-  { intro le, induction le,
+  { intro le,
+    induction le;
+    introv Hseen Hinj Hle Hss Hle';
+    simp [transl_to_stmt, transl_to_exp] at Hle,
+
     case lowstar.exp.int Y n {
-      introv Hle Hss Hle',
-      simp [transl_to_stmt, transl_to_exp] at Hle,
       opt_inv Hle,
       cases Hss,
       cases a, cases Hle', cases a_1, -- FIXME naming
       constructor },
     case lowstar.exp.unit {
-      introv Hle Hss Hle',
-      simp [transl_to_stmt, transl_to_exp] at Hle, opt_inv Hle,
+      opt_inv Hle,
       cases Hss, cases a, cases Hle', cases a_1, constructor },
     case lowstar.exp.loc {
-      introv Hle Hss Hle',
-      simp [transl_to_stmt, transl_to_exp] at Hle, opt_inv Hle,
+      opt_inv Hle,
       cases Hss, cases a_1, cases Hle', cases a_2, constructor },
     case lowstar.exp.var {
-      introv Hle Hss Hle',
-      simp [transl_to_stmt, transl_to_exp] at Hle, opt_inv Hle,
+      opt_inv Hle,
       cases Hss, cases a_1,
       rw [show close_vars names V (exp.var a) = v,
           by { simp [close_vars, exp_bind], rw [a_2], simp [close_vars] } ],
@@ -632,19 +651,17 @@ begin
       assumption, assumption
     },
     case lowstar.exp.subbuf {
-      introv Hle Hss Hle',
-      simp [transl_to_stmt, transl_to_exp] at Hle,
       opt_inv Hle with x1 H1 x2 H2,
       cases Hss, cases a_2, cases Hle', cases a_5,
       apply transition.star_trans,
       { steps_with_ctx (ectx.subbuf_1 ectx.here _),
         apply ih_1,
-        show eval_head_exp _ _ [stmt.return x2] _, { ok }, ok, ok
+        show eval_head_exp _ _ [stmt.return x2] _, { ok }, repeat { ok }
       },
       apply transition.star_trans,
       { steps_with_ctx (ectx.subbuf_2 (value.loc (b,n,[])) ectx.here),
         apply ih_2,
-        show eval_head_exp _ _ [stmt.return x1] _, { ok }, ok, ok
+        show eval_head_exp _ _ [stmt.return x1] _, { ok }, repeat { ok }
       },
       apply transition.star_one,
       { apply step_here_close_vars_lemma, apply astep.subbuf },
@@ -652,37 +669,73 @@ begin
     },
 
     case lowstar.exp.if_then_else {
-      introv Hle Hss Hle',
-      simp [transl_to_stmt, transl_to_exp] at Hle,
       opt_inv Hle with ss1 seen1 H1' Ha_1 x1 H1 foo bar,
       simp [transl_to_stmt] at H1', opt_inv H1' with ss2 seen2 H2' Ha_2,
       simp [transl_to_stmt] at H2', opt_inv H2',
       cases Hss /- ? -/ },
 
     case lowstar.exp.let_in {
-      introv Hle Hss Hle',
-      simp [transl_to_stmt, transl_to_exp] at Hle,
       opt_inv Hle with ss1 seen1 H1' H_a_2 x1 H1,
       simp [transl_to_stmt] at H1', opt_inv H1',
       cases Hss, cases Hle' with _ _ _ _ _ τ le1 le2 Hle1 Hle2 Hτ, clear Hle',
       dsimp at Hτ,
       -- simp [transl_typ_injective Hτ] at *,
       note hh := (transl_typ_injective Hτ), subst hh, clear Hτ, /- FIXME: rw at * -/
-      rw (back_transl_stmt_eq a_2 le2); ok; [skip, admit, admit],
+      rw (back_transl_stmt_eq a_2 le2); ok; ok,
       steps_with_ctx (ectx.let_in _ ectx.here _),
       apply ih_1; ok
     },
 
     case lowstar.exp.ignore Y e1 e2 {
-      introv Hle Hss Hle',
-      simp [transl_to_stmt, transl_to_exp] at Hle,
       opt_inv Hle with ss1 seen1 H1' H1, simp [transl_to_stmt] at H1', opt_inv H1',
       cases Hss, cases Hle', case back_stmt.ignore e1' e2' He1' He2' {
-        rw (back_transl_stmt_eq e2 e2' _ _ _ _ _ H1 He2'); ok; [skip, admit],
+        rw (back_transl_stmt_eq e2 e2' _ _ _ _ _ _ H1 He2'); ok,
         steps_with_ctx (ectx.ignore ectx.here _),
         apply ih_1; ok
       }
     },
+
+    case lowstar.exp.let_app Y τ fn e1 e2 {
+      opt_inv Hle with ss1 seen1 H1' H1, simp [transl_to_stmt] at H1', opt_inv H1',
+      cases Hss, cases Hle', case back_stmt.let_app x τ' e1' e2' Hx Hτ He1' He2' {
+        dsimp at Hx Hτ, rw (back_transl_stmt_eq e2 e2'); ok; ok,
+        rw (transl_typ_injective Hτ), clear Hτ,
+        steps_with_ctx (ectx.let_app _ _ ectx.here _),
+        apply ih_1; ok
+      }
+    },
+
+    case lowstar.exp.let_newbuf Y n e1 τ e2 {
+      opt_inv Hle with ss1 seen1 H1' H1, simp [transl_to_stmt] at H1', opt_inv H1',
+      cases Hss, cases Hle', case back_stmt.let_newbuf e1' τ' e2' Hx He1' Hτ He2' {
+        dsimp at Hx Hτ,
+        rw (transl_typ_injective Hτ), clear Hτ,
+        rw (back_transl_exp_eq e1 e1'); ok,
+        rw (back_transl_stmt_eq e2 e2'); ok; ok,
+        constructor, assumption
+      }
+    },
+
+    -- case lowstar.exp.let_readbuf Y τ e1 e2 e3 {
+    --   opt_inv Hle with ss1 seen1 H1' H1, simp [transl_to_stmt] at H1', opt_inv H1',
+    --   cases Hss, case eval_head_exp.read v Hv {
+    --   cases Hv,
+    --   -- assert Hve : (exists v_e : cstar.exp, ↑v = v_e), { existsi ↑v, refl }, cases Hve with v_e Hve,
+    --   -- rw Hve at Hle',  -- FIXME
+    --   cases Hle', case back_stmt.let_readbuf x τ' e1_1 e1_2 e1' e2' e3' Hx Hτ He1' He2' He3' {
+    --     rw (back_transl_stmt_eq e3 e3'); ok; ok,
+    --     dsimp at Hx Hτ, subst Hx, rw (transl_typ_injective Hτ), clear Hτ, -- FIXME: Hv printing
+
+
+
+    --     -- apply transition.star_trans,
+    --     -- { steps_with_ctx (ectx.let_readbuf_1 _ ectx.here _ _),
+    --     --   apply ih_1, assumption, apply transl_to_stmt_exp, assumption,
+
+
+    --     -- }
+    --   }
+    -- }},
 
     repeat { admit }
   },
